Until Type System, refactoring done

theories/Syntax/Term.v
@@ -1,12 +1,12 @@
-From Coq Require Import Classical_Prop Classes.RelationClasses Classes.Morphisms Bool.Bool Lia.
-From DeBrLevel Require Import LevelInterface OptionLevel.
+From Coq Require Import Classes.Morphisms Lia.
+From DeBrLevel Require Import LevelInterface Level OptionLevel.
 From Mecha Require Import Var Resource Typ.
 Import VarNotations ResourceNotations TypNotations.
 
 
 (** * Syntax - Term
 
-  Wormholes's syntax is an extended version of the standard lambda calculus with pair, projections, fixpoint, ground value, denoted [()], and arrow primitives (arr,first and comp). In addition, the language introduces [rsf] and [wormhole]. The former access to the environment and allows interaction with it. The latter creates local resources.
+  Wormhole's terms are those of the arrow calculus with two additional arrow primitives named [rsf] and [wormhole] that respectively represent an interaction with the environment and a [let...in] structure for resource names and reactive expression. The definition relies on [Resource.v].
 *)
 
 (** ** Module - Term *)
@@ -19,15 +19,15 @@ Open Scope typ_scope.
 
 (** **** Type 
 
-  The syntax is an usual lambda-calculus, with arrow primitives (arr, first and comp) as well as two additional arrow primitives named [rsf] and [wormhole] that respectively represent an interaction with the environment and a [let...in] structure for resource names and reactive expression.
+  Wormholes's syntax is an extended version of the standard lambda calculus with pair, projections, fixpoint, ground value, denoted [()], and arrow primitives (arr,first and comp). In addition, the language introduces [rsf] and [wormhole]. The former access to the environment and allows interaction with it. The latter creates local resources.
 *)
 Inductive raw : Type :=
   | tm_unit   : raw
-  | tm_fix    : raw
   | tm_var (x : variable) : raw
   | tm_abs (x : variable) (t : raw) : raw
   | tm_app  (t1 t2 : raw) : raw
   | tm_pair (t1 t2 : raw) : raw
+  | tm_fix   (t : raw) : raw
   | tm_fst   (t : raw) : raw
   | tm_snd   (t : raw) : raw
   | tm_arr   (t : raw) : raw
@@ -42,13 +42,14 @@ Definition eq := @eq t.
 
 (** **** Shift function 
 
-  The [shift] function takes a lower bound [lb] a natural [k] and a term [t], and produces a term [t'] where all resources [r] greater or equal to [lb] in [t] are incremented by [k]. The others are left unchanged.
+  The [shift] function takes a lower bound [lb] a natural [k] and a term [t], and produces a term [t'] where all resources [r] greater or equal to [lb] in [t] are incremented by [k]. The others are left unchanged. It is denoted [[⧐ lb – k] t].
 *)
-Fixpoint shift (lb : nat) (k : nat) (e : t) : t := 
+Fixpoint shift (lb : lvl) (k : lvl) (e : t) : t := 
   match e with
   | tm_rsf r => tm_rsf ([⧐ lb – k] r)
 
   | tm_abs x t0 => tm_abs x (shift lb k t0)
+  | tm_fix t0   => tm_fix   (shift lb k t0)
   | tm_fst t0   => tm_fst   (shift lb k t0)
   | tm_snd t0   => tm_snd   (shift lb k t0)
   | tm_arr t0   => tm_arr   (shift lb k t0)
@@ -63,108 +64,82 @@ Fixpoint shift (lb : nat) (k : nat) (e : t) : t :=
   end
 .
 
-(*========================= STOP ===============================*)
+(** **** Multi shift function 
 
-Definition multi_shift (lbs : list nat) (ks : list nat) (t : t) :=
-  List.fold_right (fun (x : nat * nat) acc => let (lb,k) := x in shift lb k acc) t (List.combine lbs ks).
+  As done in [Resource.v], [Resources.v] and [Typ.v], we define a [multi_shift] function that applies [n] shifts for two lists [lbs] and [ks] of length [n].
+*)
+Definition multi_shift (lbs : list lvl) (ks : list lvl) (t : t) :=
+  List.fold_right (fun lbk acc => shift (fst lbk) (snd lbk) acc) t (List.combine lbs ks).
 
 
-(** **** Valid function 
+(** **** Valid property 
 
-  A term is valid if all their types and resources contained in it are valid.
-  However the lower bound is incremented by 2 when we go through a [wormhole] structure because
-  2 virtuals resources exist in it. This is why we can define terms fully constained. Indeed, the lemma
-  [shift_valid_refl] can be hold in this case.
-
+  Defined as an inductive property and denoted [(⊩)], the well-formed property, named [valid], takes a level [k] called the well-formedness level and states that all resource names in the type are well-formed under [k]. Contrary to the property defined in [Typ.v], it is not exactly true because of bound resource names. Indeed, [k] may increase during the descent into the sub-term. It happens when
+  we go through a [wormhole] term. It is the reactive binder that binds two resource names. If 
+  [k ⊩ wormhole(t1;t2)] then its local resource names will be [k] and [S k]. Consequently, the
+  well-formedness level [k] becomes [k + 2] in [t2]. A direct consequence the definition is that
+ [shift_valid_refl] cannot hold anymore.
 <<
-We can state that:
+We recall the lemma below.
 
-valid 0 wormhole(unit;rsf[0]) <-> valid 0 unit /\ valid 2 rsf[0]
+Lemma shift_valid_refl (lb k : lvl) (t : t) : valid lb t -> (shift lb k t) = t.
 
-but
+Suppose t equals to wormhole(unit;rsf[0]), lb equals to 0 and k equals to 3. We know that: 
 
-            (shift 0 3 wormhole(unit;rsf[0])) ≠ wormhole(unit;rsf[0])
-wormhole((shift 0 3 unit);(shift 0 3 rsf[0])) ≠ wormhole(unit;rsf[0])
-                        wormhole(unit;rsf[3]) ≠ wormhole(unit;rsf[0])
+0 ⊩ wormhole(unit;rsf[0])
+
+However, 
+
+               ([⧐ 0 – 3] wormhole(unit;rsf[0])) ≠ wormhole(unit;rsf[0])
+  wormhole(([⧐ 0 – 3] unit);([⧐ 0 – 3] rsf[0])) ≠ wormhole(unit;rsf[0])
+                           wormhole(unit;rsf[3]) ≠ wormhole(unit;rsf[0])
 >>
 *)
-Inductive valid' : nat -> t -> Prop :=
-  | vΛ_unit : forall k, valid' k tm_unit
-  | vΛ_var : forall k x, valid' k (tm_var x)
-  | vΛ_fix : forall k, valid' k tm_fix
-  | vΛ_app : forall k t1 t2, valid' k t1 -> valid' k t2 -> valid' k (tm_app t1 t2)
-  | vΛ_abs : forall k x t, valid' k t -> valid' k (tm_abs x t)
-  
-  | vΛ_pair : forall k t1 t2, valid' k t1 -> valid' k t2 -> valid' k (tm_pair t1 t2)
-  | vΛ_fst  : forall k t, valid' k t -> valid' k (tm_fst t) 
-  | vΛ_snd  : forall k t, valid' k t -> valid' k (tm_snd t)
-  
-  | vΛ_arr   : forall k t, valid' k t -> valid' k (tm_arr t)
-  | vΛ_first : forall k t, valid' k t -> valid' k (tm_first t)
-  | vΛ_comp  : forall k t1 t2, valid' k t1 -> valid' k t2 -> valid' k (tm_comp t1 t2)
-  | vΛ_rsf : forall k r, (k ⊩ r)%r ->  valid' k (tm_rsf r)
-  | vΛ_wh  : forall k t1 t2, valid' k t1 -> valid' (S (S k)) t2 -> valid' k (tm_wh t1 t2)
+Inductive valid' : lvl -> t -> Prop :=
+  | vΛ_unit (k : lvl) : valid' k tm_unit
+  | vΛ_var  (k : lvl) (x : variable) : valid' k (tm_var x)
+  | vΛ_abs  (k : lvl) (x : variable) (t : t) : valid' k t -> valid' k (tm_abs x t)
+
+  | vΛ_app  (k : lvl) (t1 t2 : t) : valid' k t1 -> valid' k t2 -> valid' k (tm_app t1 t2)
+  | vΛ_pair (k : lvl) (t1 t2 : t) : valid' k t1 -> valid' k t2 -> valid' k (tm_pair t1 t2)
+
+  | vΛ_fix   (k : lvl) (t : t) : valid' k t -> valid' k (tm_fix t) 
+  | vΛ_fst   (k : lvl) (t : t) : valid' k t -> valid' k (tm_fst t) 
+  | vΛ_snd   (k : lvl) (t : t) : valid' k t -> valid' k (tm_snd t)
+  | vΛ_arr   (k : lvl) (t : t) : valid' k t -> valid' k (tm_arr t)
+  | vΛ_first (k : lvl) (t : t) : valid' k t -> valid' k (tm_first t)
+
+  | vΛ_rsf (k : lvl) (r : resource) : (k ⊩ r)%r ->  valid' k (tm_rsf r)
+
+  | vΛ_comp (k : lvl) (t1 t2 : t) : valid' k t1 -> valid' k t2 -> valid' k (tm_comp t1 t2)
+  | vΛ_wh   (k : lvl) (t1 t2 : t) : valid' k t1 -> valid' (S (S k)) t2 -> valid' k (tm_wh t1 t2)
 .
 
 Definition valid := valid'.
 
 #[export] Hint Constructors valid' : core.
 
-(** **** Others *)
+(** **** Value property 
 
-Inductive appears_free_in : variable -> t -> Prop :=
-  | afi_var : forall (x : variable), appears_free_in x (tm_var x)
-  
-  | afi_app1 :  forall x t1 t2, appears_free_in x t1 -> appears_free_in x (tm_app t1 t2)
-
-  | afi_app2 :  forall x t1 t2, appears_free_in x t2 -> appears_free_in x (tm_app t1 t2)
-
-  | afi_abs  :  forall x y t,
-                  y <> x  -> appears_free_in x t -> appears_free_in x (tm_abs y t) 
-
-  | afi_pair1 : forall x t1 t2, appears_free_in x t1 -> appears_free_in x (tm_pair t1 t2)
-
-  | afi_pair2 : forall x t1 t2, appears_free_in x t2 -> appears_free_in x (tm_pair t1 t2)
-
-  | afi_fst   : forall x t, appears_free_in x t -> appears_free_in x (tm_fst t)
-  | afi_snd   : forall x t, appears_free_in x t -> appears_free_in x (tm_snd t)
-  | afi_arr   : forall x t, appears_free_in x t -> appears_free_in x (tm_arr t)
-  | afi_first : forall x t, appears_free_in x t -> appears_free_in x (tm_first t)
-  
-  | afi_comp1 : forall x t1 t2, appears_free_in x t1 -> appears_free_in x (tm_comp t1 t2)
-  | afi_comp2 : forall x t1 t2, appears_free_in x t2 -> appears_free_in x (tm_comp t1 t2)
-
-  | afi_wh1 : forall x t1 t2, appears_free_in x t1 -> appears_free_in x (tm_wh t1 t2)
-  | afi_wh2 : forall x t1 t2, appears_free_in x t2 -> appears_free_in x (tm_wh t1 t2)
-.
-
-Definition closed (t : t) := forall x, ~ (appears_free_in x t).
-
+  The evaluation transition definition, available in [ET_Definition.v], needs to differentiate terms and values. Ground values are [()], abstractions and [rsf]. We also consider as value
+  pairs, and reactive terms only if all of their sub-terms are also values.
+*)
 Inductive value : t -> Prop :=
-  | v_unit  : value tm_unit
-  | v_fix  : value tm_fix
+  | v_unit : value tm_unit
+  | v_rsf (r : resource) : value (tm_rsf r)
+  | v_abs (x : variable) (t : t) : value (tm_abs x t)
 
-  | v_abs   : forall x t, value (tm_abs x t)
+  | v_arr   (v : t) : value v -> value (tm_arr v)
+  | v_first (v : t) : value v -> value (tm_first v)
 
-  | v_pair  : forall v1 v2, 
-                value v1 -> value v2 -> value (tm_pair v1 v2)
-
-  | v_arr   : forall t, value t -> value (tm_arr t)
-
-  | v_first : forall t, value t -> value (tm_first t)
-
-  | v_comp  : forall t1 t2, value t1 -> value t2 -> value (tm_comp t1 t2)
-
-  | v_rsf   : forall r, value (tm_rsf r)
-
-  | v_wh    : forall i t, value i -> value t -> value (tm_wh i t)
+  | v_pair (v1 v2 : t) : value v1 -> value v2 -> value (tm_pair v1 v2)
+  | v_comp (v1 v2 : t) : value v1 -> value v2 -> value (tm_comp v1 v2)
+  | v_wh   (v1 v2 : t) : value v1 -> value v2 -> value (tm_wh v1 v2)
 .
 
+#[export] Hint Constructors value valid' : core.
 
-#[global] 
-Hint Constructors value appears_free_in : core.
-
-(** *** Equality *)
+(** *** Property *)
 
 #[export] Instance eq_refl : Reflexive eq := _.
 #[export] Instance eq_sym : Symmetric eq := _.
@@ -174,188 +149,162 @@ Hint Constructors value appears_free_in : core.
 
 #[export] Hint Resolve eq_refl eq_sym eq_trans : core.
 
-Lemma eq_dec : forall (e e' : t), {eq e e'} + {~ eq e e'}.
+Lemma eq_dec (t1 t2 : t) : {eq t1 t2} + {~ eq t1 t2}.
 Proof.
-  unfold eq; intros e; induction e; intros e'; destruct e'; simpl; auto; 
+  unfold eq; revert t2; induction t1; intro; destruct t2; simpl; auto; 
   try (right; unfold not; intros contra; now inversion contra);
-  try (destruct (IHe1 e'1); destruct (IHe2 e'2);
+  try (destruct (IHt1_1 t2_1); destruct (IHt1_2 t2_2);
   try (right; unfold not; intros; inversion H; subst; contradiction); subst; f_equal; auto);
-  try (destruct (IHe e'); subst; try (now left); right; intro c; 
+  try (destruct (IHt1 t2); subst; try (now left); right; intro c; 
         inversion c; subst; now contradiction).
-  - destruct (Var.eqb_spec v v0); subst.
+  - destruct (Var.eqb_spec x x0); subst.
     -- now left.
     -- right; intro c; inversion c; subst; clear c; now contradiction n.
-  - destruct (Var.eqb_spec v v0); subst;
-    destruct (IHe e'); subst; try (right; intro c; inversion c; subst; now contradiction).
+  - destruct (Var.eqb_spec x x0); subst;
+    destruct (IHt1 t2); subst; try (right; intro c; inversion c; subst; now contradiction).
     now left.
   - destruct (Resource.eq_dec r r0); subst; try now left. right; intro c; inversion c; subst;
     contradiction.
 Qed.
 
-Lemma eq_leibniz : forall x y, eq x y -> x = y. Proof. auto. Qed.
+Lemma eq_leibniz (t1 t2 : t) : eq t1 t2 -> t1 = t2. 
+Proof. auto. Qed.
 
-(** *** Shift *)
+(** **** [shift] property *)
 
-Lemma shift_zero_refl : forall (lb : nat) (t : t), shift lb 0 t = t.
+Lemma shift_zero_refl (lb : lvl) (t : t) : shift lb 0 t = t.
 Proof.
-  intros lb t; induction t; simpl; f_equal; auto.
+  induction t; simpl; f_equal; auto.
   apply Resource.shift_zero_refl.
 Qed.
 
 #[export] Instance shift_eq : Proper (Logic.eq ==> Logic.eq ==> eq ==> eq) shift := _.
 
-Lemma shift_eq_iff : forall lb k t t1,
+Lemma shift_eq_iff (lb k : lvl) (t t1 : t) :
   t = t1 <-> (shift lb k t) = (shift lb k t1).
 Proof.
-  split.
-  - intros; now subst.
-  - revert lb k t1; induction t0; intros lb k t' Heq; destruct t'; 
+  split; intro Heq.
+  - now subst.
+  - revert t1 Heq; induction t; intros t' Heq; destruct t'; 
     simpl in *; try (now inversion Heq); try (inversion Heq;f_equal; eauto).
     eapply Resource.shift_eq_iff; eauto.
 Qed.
 
-Lemma shift_trans : forall lb k k' t,
-  shift lb k (shift lb k' t) = shift lb (k + k') t.
+Lemma shift_trans (lb k m : lvl) (t : t) :
+  shift lb k (shift lb m t) = shift lb (k + m) t.
 Proof.
-  intros lb k k' t; induction t; simpl; f_equal; auto.
+  induction t; simpl; f_equal; auto.
   apply Resource.shift_trans.
 Qed.
 
-Lemma shift_permute : forall lb k k' t,
-  shift lb k (shift lb k' t) = shift lb k' (shift lb k t).
+Lemma shift_permute (lb k m : lvl) (t : t) :
+  shift lb k (shift lb m t) = shift lb m (shift lb k t).
 Proof.
-  intros lb k k' t; induction t; simpl; f_equal; auto.
+  induction t; simpl; f_equal; auto.
   apply Resource.shift_permute.
 Qed.
 
-Lemma shift_not_fix_iff : forall t lb k,
-  t <> tm_fix <-> (shift lb k t) <> tm_fix.
+Lemma shift_value_iff (lb k : lvl) (t : t) : value t <-> value (shift lb k t).
 Proof.
-  intro t; induction t; intros; split; simpl; 
-  intros; intro; inversion H0;
-  try contradiction.
-Qed.
-
-Lemma shift_afi_iff : forall  t s lb k,
-  appears_free_in s t <-> appears_free_in s (shift lb k t).
-Proof. 
-  intros t; induction t; intros x lb k; split; intros HFV; simpl in *; auto;
-  try (inversion HFV; subst; constructor; auto; rewrite IHt in *; eauto);
-  inversion HFV; subst; try (constructor; apply IHt1; now eauto);
-  try (constructor; rewrite IHt1; now eauto).
-  - apply afi_app2; rewrite <- IHt2; eauto.
-  - apply afi_app2; rewrite IHt2; eauto.
-  - apply afi_pair2; now rewrite <- IHt2.
-  - apply afi_pair2; rewrite IHt2; eauto.
-  - apply afi_comp2; now rewrite <- IHt2.
-  - apply afi_comp2; rewrite IHt2; eauto.
-  - apply afi_wh2; now rewrite <- IHt2.
-  - apply afi_wh2; rewrite IHt2; eauto.
-Qed.
-
-Lemma shift_closed_iff : forall t lb k, closed t <-> closed (shift lb k t).
-Proof. 
-  unfold closed, not; intros; split; intros; apply (H x).
-  - rewrite shift_afi_iff ; eauto.
-  - rewrite shift_afi_iff in H0; eauto.
-Qed.
-
-Lemma shift_value_iff : forall t lb k, value t <-> value (shift lb k t).
-Proof.
-  intros t; induction t; split; intros; auto; simpl;
+  induction t; split; intros; auto; simpl;
   try (now inversion H); try (inversion H; subst; constructor);
   try (erewrite IHt1; now eauto); try (erewrite <- IHt1; now eauto);
   try (erewrite IHt2; now eauto); try (erewrite <- IHt2; now eauto);
   try (now apply IHt); try (erewrite IHt; eauto).
 Qed.
 
-Lemma shift_permute_1 : forall t lb k k',
-  eq (shift lb k (shift lb k' t)) (shift (lb + k) k' (shift lb k t)).
+Lemma shift_permute_1 (lb k m : lvl) (t : t) :
+  eq (shift lb k (shift lb m t)) (shift (lb + k) m (shift lb k t)).
 Proof.
-  unfold eq; intro t; induction t; simpl; intros lb k k'; f_equal; auto.
+  unfold eq; induction t; simpl; f_equal; auto.
   apply Resource.shift_permute_1.
 Qed.
 
-Lemma shift_permute_2 : forall lb lb' k k' t,
-  lb <= lb' -> eq (shift lb k (shift lb' k' t)) (shift (lb' + k) k' (shift lb k t)).
+Lemma shift_permute_2 (lb k m n : lvl) (t : t) :
+  lb <= k -> eq (shift lb m (shift k n t)) (shift (k + m) n (shift lb m t)).
 Proof.
-  unfold eq; intros lb lb' k k' t; induction t; simpl; intros; f_equal; auto.
+  unfold eq; induction t; simpl; intros; f_equal; auto.
   now apply Resource.shift_permute_2.
 Qed.
 
-Lemma shift_unfold : forall lb k k' t,
-  eq (shift lb (k + k') t) (shift (lb + k) k' (shift lb k t)). 
+Lemma shift_unfold (lb k m : lvl) (t : t) :
+  eq (shift lb (k + m) t) (shift (lb + k) m (shift lb k t)). 
 Proof.
-    intros lb k k' t; induction t; simpl; auto;
-    try (rewrite IHt1; rewrite IHt2; now reflexivity);
-    try (rewrite IHt; now reflexivity).
-    now rewrite Resource.shift_unfold.
+  induction t; simpl; auto;
+  try (rewrite IHt1; rewrite IHt2; now reflexivity);
+  try (rewrite IHt; now reflexivity).
+  now rewrite Resource.shift_unfold.
 Qed.
 
-Lemma shift_unfold_1 : forall k k' k'' t,
-    k <= k' -> k' <= k'' -> 
-    eq (shift k' (k'' - k') (shift k  (k' - k) t)) (shift k (k'' - k) t).
+Lemma shift_unfold_1 (k m n : lvl) (t : t) :
+  k <= m -> m <= n -> 
+  eq (shift m (n - m) (shift k  (m - k) t)) (shift k (n - k) t).
 Proof.
-    intros k k' k'' t Hlt Hlt'; induction t; simpl; auto;
-    try (rewrite IHt1; rewrite IHt2; now reflexivity);
-    try (rewrite IHt; now reflexivity).
-    now rewrite Resource.shift_unfold_1.
+  intros Hlekm Hlemn; induction t; simpl; auto;
+  try (rewrite IHt1; rewrite IHt2; now reflexivity);
+  try (rewrite IHt; now reflexivity).
+  now rewrite Resource.shift_unfold_1.
 Qed.
 
-(** *** Valid *)
-
+(** **** [valid] property *)
 
 #[export] Instance valid_eq : Proper (Logic.eq ==> eq ==> iff) valid := _.
 
-Lemma valid_weakening : forall k k' t, (k <= k') -> valid k t -> valid k' t.
+Lemma valid_weakening (k m : lvl) (t : t) : (k <= m) -> valid k t -> valid m t.
 Proof.
-    unfold valid; intros k k' t; generalize k k'; clear k k'; induction t; 
-    intros k k'; simpl; auto; intros Hlt Hv; try (inversion Hv; subst; now eauto).
-    - inversion Hv; subst; constructor; eapply Resource.valid_weakening; eauto.
-    - inversion Hv; subst; apply vΛ_wh.
+  unfold valid; revert k m; induction t; simpl; intros k m Hle Hvt; 
+  auto; try (inversion Hvt; subst; now eauto).
+  - inversion Hvt; subst; constructor; eapply Resource.valid_weakening; eauto.
+  - inversion Hvt; subst; apply vΛ_wh.
     -- eapply IHt1; eauto.
     -- apply IHt2 with (k := S (S k)); eauto; lia.
 Qed.
 
-Theorem shift_preserves_valid_1 : forall lb k k' t,
-    valid k t -> valid (k + k') (shift lb k' t).
+Theorem shift_preserves_valid_1 (lb k m : lvl) (t : t) :
+  valid k t -> valid (k + m) (shift lb m t).
 Proof.
-    unfold valid; intros lb k k' t; revert lb k k'; induction t; intros lb k k' Hvt; 
-    inversion Hvt; subst; simpl; auto.
-    - constructor; now apply Resource.shift_preserves_valid_1.
-    - apply vΛ_wh; auto. replace (S (S (k + k'))) with ((S (S k)) + k'); auto; lia.
+  unfold valid; revert lb k m; induction t; intros lb k m Hvt; 
+  inversion Hvt; subst; simpl; auto.
+  - constructor; now apply Resource.shift_preserves_valid_1.
+  - apply vΛ_wh; auto. 
+    replace (S (S (k + m))) with ((S (S k)) + m); auto; lia.
 Qed.
 
-Theorem shift_preserves_valid : forall k k' t,
-    valid k t -> valid (k + k') (shift k k' t).
+Theorem shift_preserves_valid (k m : lvl) (t : t) :
+  valid k t -> valid (k + m) (shift k m t).
 Proof. intros; now apply shift_preserves_valid_1. Qed. 
 
-Theorem shift_preserves_valid_zero : forall k t,
-    valid k t -> valid k (shift k 0 t).
+Theorem shift_preserves_valid_zero (k : lvl) (t : t) :
+  valid k t -> valid k (shift k 0 t).
 Proof. 
-    intros. apply shift_preserves_valid with (k' := 0) in H. 
-    replace (k + 0) with k in H; auto.
+  intro Hvt. 
+  apply shift_preserves_valid with (m := 0) in Hvt. 
+  replace (k + 0) with k in Hvt; auto.
 Qed. 
 
-Lemma shift_preserves_valid_gen : forall lb lb' k k' t,
-    k <= k' -> lb <= lb' -> k <= lb -> k' <= lb' -> k' - k = lb' - lb -> 
-    valid lb t -> valid lb' (shift k (k' - k) t).
+Lemma shift_preserves_valid_gen (lb k m n : lvl) (t : t) :
+    m <= n -> lb <= k -> m <= lb -> n <= k -> n - m = k - lb -> 
+    valid lb t -> valid k (shift m (n - m) t).
 Proof.
-    intros lb lb' k k' t; revert k k' lb lb'; induction t; intros; simpl; inversion H4; subst; 
-    constructor; eauto; try (apply IHt1 with lb; now auto);
-    try (apply IHt2 with lb; now auto); try (apply IHt with lb; now auto).
-    - apply Resource.shift_preserves_valid_gen with lb; auto.
-    - apply IHt2 with (lb := S (S lb)); auto; lia.
+  revert lb k m n; induction t; 
+  intros lb k m n Hlemn Hlelbk Hlemlb Hlenk Heq Hvt; simpl; 
+  inversion Hvt; subst; constructor;
+  try (apply IHt1 with lb; now auto);
+  try (apply IHt2 with lb; now auto); try (apply IHt with lb; now auto).
+  - apply Resource.shift_preserves_valid_gen with lb; auto.
+  - apply IHt2 with (lb := S (S lb)); auto; lia.
 Qed.
 
-Lemma shift_preserves_valid_2 : forall lb lb' t,
-    lb <= lb' -> valid lb t -> 
-    valid lb' (shift lb (lb' - lb) t).
-Proof. intros. eapply shift_preserves_valid_gen; eauto. Qed.
+Lemma shift_preserves_valid_2 (m n : lvl) (t : t) :
+  m <= n -> valid m t -> valid n (shift m (n - m) t).
+Proof. 
+  intros Hle Hvt. 
+  eapply shift_preserves_valid_gen; eauto. 
+Qed.
 
-(** *** Multi Shift *)
+(** **** [multi_shift] property *)
 
-Lemma multi_shift_unit lbs ks :
+Lemma multi_shift_unit (lbs ks : list lvl) :
   multi_shift lbs ks tm_unit = tm_unit.
 Proof. 
   unfold multi_shift; revert ks.
@@ -364,181 +313,129 @@ Proof.
   now rewrite IHlbs.
 Qed.
 
-Lemma multi_shift_fix lbs ks :
-  multi_shift lbs ks tm_fix = tm_fix.
-Proof. 
-  unfold multi_shift. revert ks.
-  induction lbs.
-  - simpl; intros; reflexivity.
-  - simpl; intros; destruct ks.
-    -- simpl; reflexivity.
-    -- simpl. rewrite IHlbs. now simpl.
-Qed.
-
-Lemma multi_shift_var lbs ks : forall x,
+Lemma multi_shift_var (lbs ks : list lvl) (x : variable) :
   multi_shift lbs ks (tm_var x) = tm_var x.
 Proof. 
-  unfold multi_shift. revert ks.
-  induction lbs.
-  - simpl; intros; reflexivity.
-  - simpl; intros; destruct ks.
-    -- simpl; reflexivity.
-    -- simpl. rewrite IHlbs. now simpl.
+  unfold multi_shift; revert ks.
+  induction lbs; simpl; intro ks; auto.
+  destruct ks; simpl; auto.
+  now rewrite IHlbs. 
 Qed.
 
-Lemma multi_shift_rsf lbs ks : forall r,
+Lemma multi_shift_rsf (lbs ks : list lvl) (r : resource) :
   multi_shift lbs ks (tm_rsf r) = tm_rsf ([⧐⧐ lbs – ks] r).
 Proof. 
-  unfold multi_shift. revert ks.
-  induction lbs.
-  - simpl; intros; reflexivity.
-  - simpl; intros; destruct ks.
-    -- simpl; reflexivity.
-    -- simpl. rewrite IHlbs. now simpl.
+  unfold multi_shift; revert ks.
+  induction lbs; simpl; intro ks; auto.
+  destruct ks; simpl; auto.
+  now rewrite IHlbs.
 Qed.
 
-Lemma multi_shift_app lbs ks : forall t1 t2,
+Lemma multi_shift_app (lbs ks : list lvl) (t1 t2 : t) :
   multi_shift lbs ks (tm_app t1 t2) = tm_app (multi_shift lbs ks t1) (multi_shift lbs ks t2).
 Proof. 
-  unfold multi_shift. revert ks.
-  induction lbs.
-  - simpl; intros; reflexivity.
-  - simpl; intros; destruct ks.
-    -- simpl; reflexivity.
-    -- simpl. rewrite IHlbs. now simpl.
+  unfold multi_shift; revert ks; induction lbs; intro ks; simpl; auto.
+  destruct ks; simpl; auto; now rewrite IHlbs.
 Qed.
 
-Lemma multi_shift_pair lbs ks : forall t1 t2,
+Lemma multi_shift_pair (lbs ks : list lvl) (t1 t2 : t) :
   multi_shift lbs ks (tm_pair t1 t2) = tm_pair (multi_shift lbs ks t1) (multi_shift lbs ks t2).
 Proof. 
-  unfold multi_shift. revert ks.
-  induction lbs.
-  - simpl; intros; reflexivity.
-  - simpl; intros; destruct ks.
-    -- simpl; reflexivity.
-    -- simpl. rewrite IHlbs. now simpl.
+  unfold multi_shift; revert ks; induction lbs; intro ks; simpl; auto.
+  destruct ks; simpl; auto; now rewrite IHlbs.
 Qed.
 
-Lemma multi_shift_comp lbs ks : forall t1 t2,
+Lemma multi_shift_comp (lbs ks : list lvl) (t1 t2 : t) :
   multi_shift lbs ks (tm_comp t1 t2) = tm_comp (multi_shift lbs ks t1) (multi_shift lbs ks t2).
 Proof. 
-  unfold multi_shift. revert ks.
-  induction lbs.
-  - simpl; intros; reflexivity.
-  - simpl; intros; destruct ks.
-    -- simpl; reflexivity.
-    -- simpl. rewrite IHlbs. now simpl.
+  unfold multi_shift; revert ks; induction lbs; intro ks; simpl; auto.
+  destruct ks; simpl; auto; now rewrite IHlbs.
 Qed.
 
-Lemma multi_shift_wh lbs ks : forall t1 t2,
+Lemma multi_shift_wh (lbs ks : list lvl) (t1 t2 : t) :
   multi_shift lbs ks (tm_wh t1 t2) = tm_wh (multi_shift lbs ks t1) (multi_shift lbs ks t2).
 Proof. 
-  unfold multi_shift. revert ks.
-  induction lbs.
-  - simpl; intros; reflexivity.
-  - simpl; intros; destruct ks.
-    -- simpl; reflexivity.
-    -- simpl. rewrite IHlbs. now simpl.
+  unfold multi_shift; revert ks; induction lbs; intro ks; simpl; auto.
+  destruct ks; simpl; auto; now rewrite IHlbs.
 Qed.
 
-Lemma multi_shift_fst lbs ks : forall t1,
-  multi_shift lbs ks (tm_fst t1) = tm_fst (multi_shift lbs ks t1).
+Lemma multi_shift_fix (lbs ks : list lvl) (t : t) :
+  multi_shift lbs ks (tm_fix t) = tm_fix (multi_shift lbs ks t).
 Proof. 
-  unfold multi_shift. revert ks.
-  induction lbs.
-  - simpl; intros; reflexivity.
-  - simpl; intros; destruct ks.
-    -- simpl; reflexivity.
-    -- simpl. rewrite IHlbs. now simpl.
+  unfold multi_shift; revert ks; induction lbs; intro ks; simpl; auto.
+  destruct ks; simpl; auto; now rewrite IHlbs.
 Qed.
 
-Lemma multi_shift_snd lbs ks : forall t1,
-  multi_shift lbs ks (tm_snd t1) = tm_snd (multi_shift lbs ks t1).
+Lemma multi_shift_fst (lbs ks : list lvl) (t : t) :
+  multi_shift lbs ks (tm_fst t) = tm_fst (multi_shift lbs ks t).
 Proof. 
-  unfold multi_shift. revert ks.
-  induction lbs.
-  - simpl; intros; reflexivity.
-  - simpl; intros; destruct ks.
-    -- simpl; reflexivity.
-    -- simpl. rewrite IHlbs. now simpl.
+  unfold multi_shift; revert ks; induction lbs; intro ks; simpl; auto.
+  destruct ks; simpl; auto; now rewrite IHlbs.
 Qed.
 
-Lemma multi_shift_arr lbs ks : forall t1,
-  multi_shift lbs ks (tm_arr t1) = tm_arr (multi_shift lbs ks t1).
+Lemma multi_shift_snd (lbs ks : list lvl) (t : t) :
+  multi_shift lbs ks (tm_snd t) = tm_snd (multi_shift lbs ks t).
 Proof. 
-  unfold multi_shift. revert ks.
-  induction lbs.
-  - simpl; intros; reflexivity.
-  - simpl; intros; destruct ks.
-    -- simpl; reflexivity.
-    -- simpl. rewrite IHlbs. now simpl.
+  unfold multi_shift; revert ks; induction lbs; intro ks; simpl; auto.
+  destruct ks; simpl; auto; now rewrite IHlbs.
 Qed.
 
-Lemma multi_shift_abs lbs ks : forall x t1,
-  multi_shift lbs ks (tm_abs x t1) = tm_abs x (multi_shift lbs ks t1).
+Lemma multi_shift_arr (lbs ks : list lvl) (t : t) :
+  multi_shift lbs ks (tm_arr t) = tm_arr (multi_shift lbs ks t).
 Proof. 
-  unfold multi_shift. revert ks.
-  induction lbs.
-  - simpl; intros; reflexivity.
-  - simpl; intros; destruct ks.
-    -- simpl; reflexivity.
-    -- simpl. rewrite IHlbs. now simpl.
+  unfold multi_shift; revert ks; induction lbs; intro ks; simpl; auto.
+  destruct ks; simpl; auto; now rewrite IHlbs.
 Qed.
 
-Lemma multi_shift_first lbs ks : forall t1,
-  multi_shift lbs ks (tm_first t1) = tm_first (multi_shift lbs ks t1).
+Lemma multi_shift_abs (lbs ks : list lvl) (x : variable) (t : t) :
+  multi_shift lbs ks (tm_abs x t) = tm_abs x (multi_shift lbs ks t).
 Proof. 
-  unfold multi_shift. revert ks.
-  induction lbs.
-  - simpl; intros; reflexivity.
-  - simpl; intros; destruct ks.
-    -- simpl; reflexivity.
-    -- simpl. rewrite IHlbs. now simpl.
+  unfold multi_shift; revert ks; induction lbs; intro ks; simpl; auto.
+  destruct ks; simpl; auto; now rewrite IHlbs.
 Qed.
 
-Lemma multi_shift_nil_l ks : forall t,
-  multi_shift nil ks t = t.
-Proof. intro. unfold multi_shift; now simpl. Qed.
-
-Lemma multi_shift_nil_r lbs : forall t,
-  multi_shift lbs nil t = t.
+Lemma multi_shift_first (lbs ks : list lvl) (t : t) :
+  multi_shift lbs ks (tm_first t) = tm_first (multi_shift lbs ks t).
 Proof. 
-  intro. unfold multi_shift; destruct lbs; reflexivity. 
+  unfold multi_shift; revert ks; induction lbs; intro ks; simpl; auto.
+  destruct ks; simpl; auto; now rewrite IHlbs.
 Qed.
 
-Lemma multi_shift_nil : forall t,
-  multi_shift nil nil t = t.
-Proof. 
-  intro. unfold multi_shift; reflexivity. 
-Qed.
+Lemma multi_shift_nil_l (ks : list lvl) (t : t) : multi_shift nil ks t = t.
+Proof. now unfold multi_shift; simpl. Qed.
 
-Lemma multi_shift_cons lb k lbs ks t:
+Lemma multi_shift_nil_r (lbs : list lvl) (t : t) : multi_shift lbs nil t = t.
+Proof. now unfold multi_shift; destruct lbs. Qed.
+
+Lemma multi_shift_nil (t : t) : multi_shift nil nil t = t.
+Proof. now unfold multi_shift. Qed.
+
+Lemma multi_shift_cons (lb k : lvl) (lbs ks : list lvl) (t : t) :
   multi_shift (lb :: lbs) (k :: ks) t = shift lb k (multi_shift lbs ks t).
-Proof.
-  unfold multi_shift; simpl; reflexivity.
-Qed.
+Proof. now unfold multi_shift. Qed.
 
-Lemma multi_shift_value_iff lbs ks t: 
+Lemma multi_shift_value_iff (lbs ks : list lvl) (t : t) : 
   value t <-> value (multi_shift lbs ks t).
 Proof.
-  split.
-  - revert ks t; induction lbs; intros;
-    unfold multi_shift in *; simpl in *; auto.
-    destruct ks; simpl in *; auto.
-    apply shift_value_iff. now apply IHlbs.
-  - revert ks t; induction lbs; intros;
-    unfold multi_shift in *; simpl in *; auto.
-    destruct ks; simpl in *; auto.
-    apply shift_value_iff in H. 
-    eapply IHlbs; eauto.
+  split; revert ks t; induction lbs; simpl; intros ks t Hvt; auto.
+  - destruct ks; simpl in *; auto.
+    rewrite multi_shift_cons.
+    apply shift_value_iff. 
+    now apply IHlbs.
+  - destruct ks; simpl in *; auto.
+    rewrite multi_shift_cons in Hvt.
+    apply shift_value_iff in Hvt. 
+    now apply IHlbs in Hvt.
 Qed.
-
 
 End Term.
 
 (** ---- *)
 
-(** * Syntax - Optional Term *)
+(** * Syntax - Optional Term 
+
+  In the temporal transition, we need to represent potential output. Thanks to the [DeBrLevel] library, we do not have to prove properties that handle level because [OptionLevel] already exists.
+*)
 
 (** ** Module - Optional Term *)
 Module OptTerm <: IsLvlETWL := IsLvlOptETWL Term.
@@ -560,48 +457,51 @@ Definition Λₒ := OptTerm.t.
 
 Coercion Term.tm_var : variable >-> Term.raw.
 Notation "value( t )" := (Term.value t) (at level 20, no associativity).
-Notation "cl( t )" := (Term.closed t) (at level 20, no associativity).
-Notation "'isFV(' r ',' t ')'" := (Term.appears_free_in r t) (at level 40, t custom wh).
+(* Notation "cl( t )" := (Term.closed t) (at level 20, no associativity). *)
+(* Notation "'isFV(' r ',' t ')'" := (Term.appears_free_in r t) (at level 40, t custom wh). *)
 
-Notation "x y"     := (Term.tm_app x y) (in custom wh at level 70, left associativity).
-Notation "\ x , y" := (Term.tm_abs x y) (in custom wh at level 90, 
-                                                    x at level 99, y custom wh at level 99, 
-                                                    left associativity).
+Notation "t1 t2"     := (Term.tm_app t1 t2) (in custom wh at level 70, left associativity).
+Notation "\ x , t" := (Term.tm_abs x t) 
+                      (in custom wh at level 90, x at level 99, t custom wh at level 99, 
+                       left associativity).
 Notation "'unit'" := (Term.tm_unit) (in custom wh at level 0).
-Notation "'Fix'" := (Term.tm_fix) (in custom wh at level 0).
-Notation "⟨ x ',' y ⟩" := (Term.tm_pair x y) (in custom wh at level 0, 
-                                                      x custom wh at level 99, 
-                                                      y custom wh at level 99).
+Notation "⟨ t1 ',' t2 ⟩" := (Term.tm_pair t1 t2) 
+                          (in custom wh at level 0, t1 custom wh at level 99, 
+                           t2 custom wh at level 99).
+
+Notation "'Fix' t"   := (Term.tm_fix t) (in custom wh at level 0).
 Notation "t '.fst'"  := (Term.tm_fst t) (in custom wh at level 0).
 Notation "t '.snd'"  := (Term.tm_snd t) (in custom wh at level 0).
-Notation "'arr(' f ')'"    := (Term.tm_arr f) (in custom wh at level 0, 
-                                                      f custom wh at level 99,
-                                                      no associativity).
-Notation "'first(' sf ')'" := (Term.tm_first sf) (in custom wh at level 0).
-Notation " sf1 '>>>' sf2 " := (Term.tm_comp sf1 sf2) (in custom wh at level 60, 
-                                                                          left associativity).
-Notation "'rsf[' r ']'"    := (Term.tm_rsf r) (in custom wh at level 0,  
-                                                      r constr, no associativity).
-Notation "'wormhole(' i ';' sf ')'" :=  (Term.tm_wh i sf ) (in custom wh at level 23,
-                                                                  i custom wh, 
-                                                                  sf custom wh, 
-                                                                  no associativity).
 
-Notation "'[⧐' lb '–' k ']' t" := (Term.shift lb k t) 
-  (in custom wh at level 45, right associativity) : term_scope.
+Notation "'rsf[' r ']'" := (Term.tm_rsf r) (in custom wh at level 0, r constr, no associativity).
+
+Notation "'arr(' t ')'"   := (Term.tm_arr t) 
+                             (in custom wh at level 0, t custom wh at level 99, no associativity).
+Notation "'first(' t ')'" := (Term.tm_first t) (in custom wh at level 0).
+Notation " t1 '>>>' t2 "  := (Term.tm_comp t1 t2) (in custom wh at level 60, left associativity).
+Notation "'wormhole(' t1 ';' t2 ')'" := (Term.tm_wh t1 t2) 
+                                        (in custom wh at level 23, t1 custom wh, t2 custom wh, 
+                                         no associativity).
+
+Notation "'[⧐' lb '–' k ']' t"   := (Term.shift lb k t) 
+                                     (in custom wh at level 45, right associativity) : term_scope.
 Notation "'[⧐⧐' lb '–' k ']' t" := (Term.multi_shift lb k t) 
-  (in custom wh at level 45, right associativity) : term_scope.
+                                    (in custom wh at level 45, right associativity) : term_scope.
 Notation "'[⧐' lb '–' k ']' t" := (OptTerm.shift lb k t) 
-  (in custom wh at level 45, right associativity) : opt_term_scope.
+                                   (in custom wh at level 45, right associativity) : opt_term_scope.
 
-Infix "⊩"  := Term.valid (at level 20, no associativity) : term_scope.   
+Infix "⊩" := Term.valid (at level 20, no associativity) : term_scope.   
 Infix "⊩" := OptTerm.valid (at level 20, no associativity) : opt_term_scope.   
-
-Infix "="  := Term.eq : term_scope.
-Infix "="  := OptTerm.eq : opt_term_scope.
+Infix "=" := Term.eq : term_scope.
+Infix "=" := OptTerm.eq : opt_term_scope.
 
 
 (** *** Morphism *)
+Import Term.
+
 #[export] Instance term_leibniz_eq : Proper Logic.eq Term.eq := _.
+#[export] Instance term_valid_proper :  Proper (Level.eq ==> eq ==> iff) valid := _.
+#[export] Instance term_shift_proper : Proper (Level.eq ==> Level.eq ==> eq ==> eq) shift := shift_eq.
+#[export] Instance term_multi_shift_proper : Proper (Logic.eq ==> Logic.eq ==> eq ==> Logic.eq) multi_shift := _.
 
 End TermNotations.
