theories/Environment/RContext.v
@@ -1,0 +1,238 @@
+From Coq Require Import Lia Classes.Morphisms.
+From Mecha Require Import Typ Resource.
+From DeBrLevel Require Import LevelInterface Level MapLevelInterface MapLevel.
+Import ResourceNotations TypNotations.
+
+(** * Context - Resource Context
+
+  The type system, defined in [Type_System.v], requires two contexts: a variable context and a resource context. The former is defined in [VContext.v] and the latter is defined here. It is a map which binds resource names with pair types. We use the module [MapLvlD] defined by the library [DeBrLevel].
+*)
+
+(** ** Module - Resource Context *)
+Module RContext <: IsBdlLvlET.
+
+(** *** Definition *)
+
+Include MapLvlD.MakeBdlLvlMapLVLD PairTyp.
+Import Raw Ext.
+
+Open Scope ptyp_scope.
+
+(** *** Property *)
+
+(** **** [shift] extra property *)
+
+Lemma shift_max_key_gt (m n x : lvl) (c : t) :
+  max_key c > x <-> max_key (shift m n c) > ([⧐m – n] x)%r.
+Proof.
+  revert x; induction c using map_induction; intro y.
+  - split; intros.
+    -- rewrite max_key_Empty_spec in H0; auto. lia.
+    -- rewrite shift_Empty_spec in H0; auto.
+       rewrite max_key_Empty_spec in H0; auto. lia.
+  - split; intros.
+    -- unfold Add in *; rewrite H0 in *; clear H0.
+       apply (max_key_add_spec) with (v := e) in H as H'.
+       destruct H' as [[Heq Hle] | [Heq Hgt]].
+       + rewrite Heq in *; clear Heq.
+         rewrite (shift_in_iff m n) in H.
+         apply (max_key_add_spec) with (v := <[ [⧐m – n] e ]>) in H as H''.
+         destruct H'' as [[Heq Hle'] | [Heq Hgt']].
+         ++ rewrite shift_add_spec. 
+            rewrite Heq.
+            unfold Level.shift.
+            destruct (Level.leb_spec m x); destruct (Level.leb_spec m y); lia.
+         ++ rewrite <- IHc1 in Hgt'. lia.
+       + rewrite IHc1 in Hgt.
+         rewrite shift_add_spec.
+         rewrite max_key_add_lt_spec; auto.
+         ++ now rewrite <- IHc1; rewrite <- Heq.
+         ++ now rewrite <- shift_in_iff.
+    -- unfold Add in *; rewrite H0 in *; clear H0.
+       rewrite shift_add_spec in *.
+       apply (max_key_add_spec) with (v := e) in H as H'.
+       destruct H' as [[Heq Hle] | [Heq Hgt]].
+       + rewrite Heq in *; clear Heq.
+         rewrite (shift_in_iff m n) in H.
+         apply (max_key_add_spec) with (v := <[ [⧐m – n] e ]>) in H as H''.
+         destruct H'' as [[Heq Hle'] | [Heq Hgt']].
+         ++ rewrite Heq in *.
+            unfold Level.shift in *.
+            destruct (Level.leb_spec m x); destruct (Level.leb_spec m y); lia.
+         ++ rewrite <- IHc1 in Hgt'. lia.
+       + rewrite IHc1 in Hgt.
+         rewrite max_key_add_lt_spec in H1; auto.
+         ++ now rewrite Heq; rewrite IHc1.
+         ++ now rewrite <- shift_in_iff.
+Qed. 
+
+Lemma shift_max_key_le (m n : Lvl.t) (c1 : t) :
+  max_key c1 <= max_key (shift m n c1).
+Proof.
+  induction c1 using map_induction.
+  - now rewrite shift_Empty_spec.
+  - unfold Add in H0; rewrite H0; clear H0. 
+    rewrite shift_add_spec.
+    apply (max_key_add_spec) with (v := e) in H as H'.
+    rewrite (shift_in_iff m n) in H.
+    apply (max_key_add_spec) with (v := <[ [⧐m – n] e ]>) in H as H''.
+    destruct H' as [[Heq Hle] | [Heq Hgt]].
+    -- rewrite Heq; clear Heq.
+       destruct H'' as [[Heq Hle'] | [Heq Hgt']].
+       + rewrite Heq; clear Heq.
+         unfold Level.shift; destruct (Level.leb m x); lia.
+       + rewrite Heq; clear Heq. 
+         rewrite <- shift_max_key_gt in Hgt'.
+         lia.
+    -- rewrite Heq; clear Heq.
+       destruct H'' as [[Heq Hle'] | [Heq Hgt']].
+       + rewrite Heq; clear Heq. lia.
+       + now rewrite Heq; clear Heq.
+Qed.
+       
+Lemma shift_new_key_le (m n : Lvl.t) (c1 : t) :
+  new_key c1 <= new_key (shift m n c1).
+Proof.
+  unfold new_key; destruct (is_empty c1) eqn:Hemp.
+  - lia.
+  - destruct (is_empty (shift m n c1)) eqn:Hemp'.
+    -- apply is_empty_2 in Hemp'. 
+       rewrite <- (shift_Empty_iff m n) in Hemp'.
+       apply is_empty_1 in Hemp'.
+       rewrite Hemp in Hemp'; now inversion Hemp'.
+    -- assert (max_key c1 <= max_key (shift m n c1)).
+       + apply shift_max_key_le.
+       + lia.
+Qed.
+
+
+(** **** Wormholes specification *)
+
+Lemma max_key_wh_spec : forall (m : t) (v v' : πΤ),
+  max_key (add (S (S (max_key m))) v (add (S (max_key m)) v' m)) = S (S (max_key m)).
+Proof.
+  intros m v v'.
+  apply max_key_add_ge_spec.
+  - apply max_key_notin_spec. 
+    rewrite max_key_add_ge_spec; auto.
+    apply max_key_notin_spec; auto.
+  - rewrite max_key_add_ge_spec; auto.
+    apply max_key_notin_spec; auto.
+Qed.
+
+Lemma new_key_wh_spec : forall (m : t) (v v' : πΤ),
+  new_key (add (S (new_key m)) v (add (new_key m) v' m)) = S (S (new_key m)).
+Proof.
+  intros m v v'; unfold new_key; 
+  rewrite is_empty_add_spec; destruct (is_empty m) eqn:Heq.
+  - rewrite max_key_add_ge_spec; auto.
+    -- apply is_empty_iff in Heq; unfold Empty,not in *; 
+      intros. destruct H. apply (Heq 1 x). apply add_mapsto_iff in H.
+      destruct H; destruct H; try lia; assumption.
+    -- rewrite max_key_add_ge_spec; auto.
+      + apply is_empty_iff in Heq. unfold Empty,not in *; 
+        intros; destruct H; now apply (Heq 0 x).
+      + rewrite max_key_Empty_spec; auto. now apply is_empty_iff.
+  - f_equal. apply max_key_wh_spec.
+Qed.
+
+Lemma valid_wh_spec : forall (m : t) (v v' : πΤ),
+  valid (new_key m) m -> 
+  (new_key m) ⊩ v -> (new_key m) ⊩ v' -> 
+  valid (S (S (new_key m))) (add (S (new_key m)) v (add (new_key m) v' m)).
+Proof.
+  intros m v v' Hvm Hvv Hvv'. 
+  apply valid_add_notin_spec.
+  - rewrite add_in_iff; intro Ha. 
+    destruct Ha as [Heq | HIn]; try lia.
+    apply new_key_notin_spec in HIn; auto.
+  - repeat split. 
+    -- unfold Resource.valid; lia.
+    -- apply PairTyp.valid_weakening with (k := new_key m); auto.
+    -- apply PairTyp.valid_weakening with (k := new_key m); auto.
+    -- apply valid_add_notin_spec.
+       + apply new_key_notin_spec; lia.
+       + repeat split.
+         ++ unfold Resource.valid; lia.
+         ++ apply PairTyp.valid_weakening with (k := new_key m); auto.
+         ++ apply PairTyp.valid_weakening with (k := new_key m); auto.
+         ++ apply valid_weakening with (k := new_key m); auto.
+Qed.
+
+(** **** Morphism *)
+
+#[export] Instance in_rctx : Proper (Logic.eq ==> eq ==> iff) In.
+Proof. intros x y Heqx c c' Heqc; subst; now rewrite Heqc. Qed.
+
+#[export] Instance find_rctx : Proper (Logic.eq ==> eq ==> Logic.eq) find.
+Proof. repeat red; intros; subst. now rewrite H0. Qed.
+
+#[export] Instance Empty_rctx : Proper (eq ==> iff) Empty.
+Proof. intros c c' Heq; now rewrite Heq. Qed.
+
+#[export] Instance Add_rctx : Proper (Resource.eq ==> PairTyp.eq ==> eq ==> eq ==> iff) (@Add PairTyp.t).
+Proof. 
+  intros x x' HeqV ty ty' HeqT c c' Heq c1 c1' Heq1.
+  apply PairTyp.eq_leibniz in HeqT; subst.
+  unfold Add; now rewrite HeqV, Heq, Heq1.
+Qed.
+
+#[export] Instance add_rctx : Proper (Resource.eq ==> PairTyp.eq ==> eq ==> eq) (@add PairTyp.t).
+Proof. 
+  intros x x' HeqV ty ty' HeqT c c' Heq.
+  apply PairTyp.eq_leibniz in HeqT; subst.
+  now rewrite HeqV, Heq. 
+Qed. 
+
+End RContext.
+
+(** ---- *)
+
+(** ** Notation - Resource Context *)
+Module RContextNotations.
+
+(** *** Scope *)
+Declare Scope rcontext_scope.
+Delimit Scope rcontext_scope with rc.
+
+
+(** *** Notation *)
+Definition ℜ := RContext.t.
+
+Notation "∅" := RContext.Raw.empty (at level 0, no associativity) : rcontext_scope. 
+Notation "R '⁺'" := (RContext.Ext.new_key R) (at level 16) : rcontext_scope.
+Notation "r '∉' Re" := (~ (RContext.Raw.In r Re)) (at level 75, no associativity) : rcontext_scope. 
+Notation "'isEmpty(' Re ')'" := (RContext.Empty Re) (at level 20, no associativity) : rcontext_scope. 
+Notation "'Add'" := (RContext.Add) (at level 20, no associativity) : rcontext_scope. 
+Notation "R '⌊' x '⌋'"  := (RContext.Raw.find x R) (at level 15, x constr) : rcontext_scope.
+Notation "'max(' R ')'" := (RContext.Ext.max_key R) (at level 15) : rcontext_scope.
+Notation "⌈ x ⤆ v '⌉' R" := (RContext.Raw.add x v R) 
+                             (at level 15, x constr, v constr) : rcontext_scope.
+Notation "'[⧐' lb '–' k ']' t" := (RContext.shift lb k t) 
+                                   (at level 65, right associativity) : rcontext_scope.
+
+Infix "⊆" := RContext.Submap (at level 60, no associativity) : rcontext_scope. 
+Infix "∈" := RContext.Raw.In (at level 60, no associativity) : rcontext_scope. 
+Infix "⊩" := RContext.valid (at level 20, no associativity) : rcontext_scope.
+Infix "=" := RContext.eq : rcontext_scope.
+
+(** *** Morphisms *)
+
+Import RContext.
+
+#[export] Instance eq_equiv_rctx : Equivalence RContext.eq := Equal_equiv.
+#[export] Instance max_rctx : Proper (eq ==> Logic.eq) (RContext.Ext.max_key) := Ext.max_key_eq.
+#[export] Instance new_rctx : Proper (eq ==> Logic.eq) (Ext.new_key) := Ext.new_key_eq.
+#[export] Instance in_rctx : Proper (Logic.eq ==> eq ==> iff) (Raw.In) := _.
+#[export] Instance find_rctx : Proper (Logic.eq ==> eq ==> Logic.eq) (Raw.find) := _.
+#[export] Instance Empty_rctx : Proper (eq ==> iff) (Empty) := _.
+#[export] Instance Add_rctx : 
+  Proper (Resource.eq ==> PairTyp.eq ==> eq ==> eq ==> iff) (@RContext.Add PairTyp.t) := _.
+#[export] Instance add_rctx : 
+  Proper (Resource.eq ==> PairTyp.eq ==> eq ==> eq) (@Raw.add PairTyp.t) := _.
+#[export] Instance Submap_rctx : Proper (eq ==> eq ==> iff) Submap := _.
+#[export] Instance Submap_po : PreOrder Submap := Submap_po.
+#[export] Instance valid_eq : Proper (Logic.eq ==> eq ==> iff) valid := _.
+#[export] Instance shift_eq : Proper (Logic.eq ==> Logic.eq ==> eq ==> eq) shift := _.
+
+End RContextNotations.
