theories/Environment/VContext.v
@@ -1,0 +1,90 @@
+From Coq Require Import Classes.Morphisms.
+From Mecha Require Import Resource Typ Var.
+From DeBrLevel Require Import LevelInterface MapLevelInterface MapLevel.
+
+(** * Context - Variable Context 
+
+  The type system, defined in [Type_System.v], requires two contexts: a variable context and a resource context. The former is defined here and the latter is defined in [RContext.v]. It is a map which binds variable names with types. We use the module [MapD] defined by the library [DeBrLevel].
+*)
+
+(** ** Module - Variable Context *)
+Module VContext <: IsBdlLvlET.
+
+(** *** Definition *)
+
+Include MapD.MakeBdlLvlMapD Var Typ.
+Import Raw Ext.
+
+(** *** Property *)
+
+#[export] Instance in_vctx : Proper (Logic.eq ==> eq ==> iff) In.
+Proof. intros x y Heqx c c' Heqc; subst; now rewrite Heqc. Qed.
+
+#[export] Instance find_vctx : Proper (Logic.eq ==> eq ==> Logic.eq) find.
+Proof. repeat red; intros; subst. now rewrite H0. Qed.
+
+#[export] Instance Empty_vctx : Proper (eq ==> iff) Empty.
+Proof. intros c c' Heq; now rewrite Heq. Qed.
+
+#[export] Instance add_vctx : Proper (Var.eq ==> Typ.eq ==> eq ==> eq) (@add Typ.t).
+Proof.
+  intros x x' HeqV ty ty' HeqT c c' Heq.
+  now rewrite HeqV; rewrite HeqT; rewrite Heq.
+Qed. 
+
+#[export] Instance Add_vctx : Proper (Var.eq ==> Typ.eq ==> eq ==> eq ==> iff) (@Add Typ.t).
+Proof. 
+  intros x x' HeqV ty ty' HeqT c c' Heq c1 c1' Heq1.
+  rewrite HeqV; rewrite HeqT.
+  unfold Add.
+  now rewrite Heq,Heq1.
+Qed.
+
+End VContext.
+
+(** ---- *)
+
+(** ** Notation - Variable Context *)
+Module VContextNotations.
+
+(** *** Scope *)
+Declare Scope vcontext_scope.
+Delimit Scope vcontext_scope with vc.
+
+(** *** Notation *)
+Definition Γ := VContext.t.
+
+Notation "r '∉' G" := (~ (VContext.Raw.In r G)) (at level 75, no associativity) : vcontext_scope. 
+Notation "∅" := VContext.Raw.empty (at level 0, no associativity) : vcontext_scope. 
+Notation "'isEmpty(' G ')'" := (VContext.Empty G) 
+                                (at level 20, no associativity) : vcontext_scope. 
+Notation "'Add'" := (VContext.Add) (at level 20, no associativity) : vcontext_scope. 
+Notation "R '⌊' x '⌋'"  := (VContext.Raw.find x R) (at level 15, x constr) : vcontext_scope.
+Notation "⌈ x ⤆ v '⌉' R"  := (VContext.Raw.add x v R) 
+                             (at level 15, x constr, v constr) : vcontext_scope.
+Notation "'[⧐' lb '–' k ']' t" := (VContext.shift lb k t) 
+                                   (at level 65, right associativity) : vcontext_scope.
+
+Infix "⊆" := VContext.Submap (at level 60, no associativity) : vcontext_scope. 
+Infix "∈" := VContext.Raw.In (at level 60, no associativity) : vcontext_scope. 
+Infix "=" := VContext.eq : vcontext_scope.
+
+Infix "⊩" := VContext.valid (at level 20, no associativity) : vcontext_scope.
+
+(** *** Morphism *)
+
+Import VContext.
+
+#[export] Instance eq_equiv_vctx : Equivalence eq := _.
+#[export] Instance in_vctx : Proper (Logic.eq ==> eq ==> iff) (Raw.In) := _.
+#[export] Instance find_vctx : Proper (Logic.eq ==> eq ==> Logic.eq) (Raw.find) := _.
+#[export] Instance Empty_vctx : Proper (eq ==> iff) (Empty) := _.
+#[export] Instance Add_vctx : 
+  Proper (Var.eq ==> Typ.eq ==> eq ==> eq ==> iff) (@VContext.Add Typ.t) := _.
+#[export] Instance add_vctx : Proper (Var.eq ==> Typ.eq ==> eq ==> eq) (@Raw.add Typ.t) := _.
+#[export] Instance Submap_vctx : Proper (eq ==> eq ==> iff) Submap := _.
+#[export] Instance valid_vctx : Proper (Logic.eq ==> eq ==> iff) valid := _.
+#[export] Instance shift_vctx : Proper (Logic.eq ==> Logic.eq ==> eq ==> eq) shift := _.
+#[export] Instance Submap_vctx_po : PreOrder Submap := _.
+
+End VContextNotations.
