theories/Semantics/Evaluation_Transition.v
@@ -1,0 +1,237 @@
+From Coq Require Import Relations.Relation_Operators.
+From Mecha Require Import Var Resource Term.
+Import VarNotations ResourceNotations TermNotations.
+
+Open Scope term_scope.
+
+(** * Semantics - Evaluation
+
+  Wormholes’s dynamic semantics is split in three sets of transition rules: the evaluation transition which extends standard β-reduction; the functional transition, defined in [Functional_Transition.v], which performs the logical instant, and the temporal transition, defined in [Temporal_Transition.v], which corresponds to the reactivity of the program: it initializes the resources values, performs the instant via the functional transition and updates the system. In this file, we focus on the evaluation transition.
+*)
+
+(** ** Definition - Evaluation *)
+
+(** *** Substitution function 
+
+  In addition to usual substitution parameters, the [subst] function carries
+  two levels, [lb] and [k]. 
+  Consider, as an illustrating example, the following expressions valid at [0].
+<<
+wh(unit; rsf[0] >>> x) (1)
+wh(unit; rsf[0])       (2)
+>>
+  With a standard substitution, the result of substituting [x] by (2) in (1) is ill-
+  formed because of the resource [0] in (2) is captured by the wh of (1).
+<<
+  [x := (2)] wh(unit; rsf[0] >>> x)
+= wh([x := (2)] unit; [x := (2)] rsf[0] >>> x)
+= wh(unit; [x := (2)] rsf[0] >>> x)
+= wh(unit; [x := (2)] rsf[0] >>> [x := (2)] x)
+= wh(unit; rsf[0] >>> wh(unit; rsf[0]))
+>>
+  With [lb] the validity level of (2), and [k] the number of bound resources encountered, we avoid
+  this issue.
+<<
+  [x := (2) ~ 0 ≤ 0] wh(unit; rsf[0] >>> x)
+= wh([x := (2) ~ 0 ≤ 0] unit; [x := (2) ~ 0 ≤ 2] rsf[0] >>> x)
+= wh(unit; [x := (2) ~ 0 ≤ 2] rsf[0] >>> x)
+= wh(unit; [x := (2) ~ 0 ≤ 2] rsf[0] >>> [x := (2) ~ 0 ≤ 2] x)
+= wh(unit; rsf[0] >>> [⧐ₜₘ 0 ≤ 2] wh(unit; rsf[0]))
+= wh(unit; rsf[0] >>> wh([⧐ₜₘ 0 ≤ 2] unit; [⧐ₜₘ 0 ≤ 2] rsf[0]))
+= wh(unit; rsf[0] >>> wh(unit; [⧐ₜₘ 0 ≤ 2] rsf[0]))
+= wh(unit; rsf[0] >>> wh(unit; rsf[2]))
+>>
+*)
+
+Reserved Notation "'[' x ':=' v '~' lb '–' k ']' t" (in custom wh at level 66, right associativity).
+
+Fixpoint subst (lb : lvl) (k : lvl) (x : variable) (v t : Λ) : Λ :=
+  match t with
+    | Term.tm_var y => if (x =? y)%v then <[[⧐ lb – k] v]> else t 
+    | <[t1 t2]> => <[([x := v ~ lb – k]t1) ([x := v ~ lb – k]t2)]>
+    | <[\y,t0]> => if (x =? y)%v then t else <[\y,[x := v ~ lb – k]t0]>
+
+    | <[⟨t1,t2⟩]> => <[⟨([x := v ~ lb – k]t1),([x := v ~ lb – k]t2)⟩]>
+    | <[t0.fst]> => <[([x := v ~ lb – k]t0).fst]>
+    | <[t0.snd]> => <[([x := v ~ lb – k]t0).snd]>
+
+    | <[arr(t0)]> => <[arr([x := v ~ lb – k]t0)]>
+    | <[first(t0)]> => <[first([x := v ~ lb – k]t0)]>
+    | <[t1 >>> t2]> => <[([x := v ~ lb – k]t1) >>> ([x := v ~ lb – k]t2)]>
+
+    | <[wormhole(t1;t2)]> => <[wormhole([x := v ~ lb – k] t1;[x := v ~ lb – {S (S k)}] t2)]>
+
+    | _ => t
+  end
+  where "'[' x ':=' v '~' lb '–' k ']' t" := (subst lb k x v t) (in custom wh)
+.
+
+Notation "'[' x ':=' v '~' lb ']' t" := (subst lb 0 x v t) 
+                                        (in custom wh at level 66,  right associativity).
+
+
+
+(** *** Evaluation transition
+
+  The evaluation transition corresponds to a determinis-
+  tic β-reduction. We choose a small step semantics with a call-by-value evaluation
+  strategy (see Figure 6) in order to bypass capture issues for variables (in particular, 
+  reduction does not act under λ’s). Modifications on the substitution
+  affect the evaluation transition. [k] being the number of bound resources encountered, 
+  we set it to [0]. But, [lb] is the level of validity of [v], thus, it cannot be deduced. 
+  Consequently, we also need [lb] to be explicit in the evaluation transition.
+*)
+
+Reserved Notation "k '⊨' t '⟼' t1" (at level 57, t custom wh, t1 custom wh, no associativity).
+
+Inductive evaluate : lvl -> Λ -> Λ -> Prop :=
+  | eT_appv (k : lvl) (x : variable) (t v : Λ) :
+
+                         value(v) ->
+      (* ------------------------------------- ET-Appv *)
+           k ⊨ ((\x,t) v) ⟼ ([x:= v ~ k] t)
+
+  | eT_fix (k : lvl) (f : variable) (t : Λ) :
+
+      (* --------------------------------------------------- ET-Fix *)
+           k ⊨ (Fix (\f,t)) ⟼ ([f := (Fix (\f,t)) ~ k] t)
+
+  | eT_app1 (k : lvl) (t1 t1' t2 : Λ) :
+
+               k ⊨ t1 ⟼ t1' -> 
+      (* --------------------------- ET-App1 *)
+           k ⊨ (t1 t2) ⟼ (t1' t2)
+
+  | eT_app2  (k : lvl) (v t t' : Λ) :
+                    
+           value(v) -> k ⊨ t ⟼ t' -> 
+      (* ------------------------------- ET-App2 *)
+              k ⊨ (v t) ⟼ (v t') 
+
+  | eT_pair1 (k : lvl) (t1 t1' t2 : Λ) :
+
+               k ⊨ t1 ⟼ t1' -> 
+      (* --------------------------- ET-Pair1 *)
+           k ⊨ ⟨t1,t2⟩ ⟼ ⟨t1',t2⟩
+
+  | eT_pair2 (k : lvl) (v t t' : Λ) :
+
+           value(v) -> k ⊨ t ⟼ t' -> 
+      (* ------------------------------ ET-Pair2 *)
+             k ⊨ ⟨v,t⟩ ⟼ ⟨v,t'⟩
+
+  | eT_fst1 (k : lvl) (t t' : Λ) :
+
+             k ⊨ t ⟼ t' -> 
+      (* ----------------------- ET-Fst1 *)
+           k ⊨ t.fst ⟼ t'.fst
+
+  | eT_fstv (k : lvl) (v1 v2 : Λ) :
+
+           value(v1) -> value(v2) -> 
+      (* ----------------------------- ET-Fstv *)
+            k ⊨ ⟨v1,v2⟩.fst ⟼ v1
+
+  | eT_snd1 (k : lvl) (t t' : Λ) :
+
+               k ⊨ t ⟼ t' -> 
+      (* ----------------------- ET-Snd1 *)
+           k ⊨ t.snd ⟼ t'.snd
+
+  | eT_sndv (k : lvl) (v1 v2 : Λ) :
+
+           value(v1) -> value(v2) -> 
+      (* ----------------------------- ET-Sndv *)
+            k ⊨ ⟨v1,v2⟩.snd ⟼ v2
+                            
+  | eT_comp1 (k : lvl) (t1 t1' t2 : Λ) :
+
+                 k ⊨ t1 ⟼ t1' -> 
+      (* ------------------------------- ET-Comp1 *)
+           k ⊨ t1 >>> t2 ⟼ t1' >>> t2
+
+  | eT_comp2 (k : lvl) (v t t' : Λ) :
+                      
+           value(v) -> k ⊨ t ⟼ t' -> 
+      (* ------------------------------- ET-Comp2 *)
+             k ⊨ v >>> t ⟼ v >>> t'
+
+  | eT_arr (k : lvl) (t t' : Λ) :
+
+               k ⊨ t ⟼ t' -> 
+      (* ------------------------- ET-Arr *)
+           k ⊨ arr(t) ⟼ arr(t')
+
+  | eT_first (k : lvl) (t t' : Λ) :
+                
+                 k ⊨ t ⟼ t' -> 
+      (* ----------------------------- ET-First *)
+           k ⊨ first(t) ⟼ first(t')
+
+  | eT_wh1 (k : lvl) (t1 t1' t2 : Λ) :
+
+                        k ⊨ t1 ⟼ t1' -> 
+      (* ------------------------------------------- ET-Wh1 *)
+           k ⊨ wormhole(t1;t2) ⟼ wormhole(t1';t2)
+
+  | eT_wh2 (k : lvl) (v t t' : Λ) :
+
+           value(v) -> (S (S k)) ⊨ t ⟼ t' -> 
+      (* ----------------------------------------- ET-Wh2 *)
+           k ⊨ wormhole(v;t) ⟼ wormhole(v;t')
+
+where "k '⊨' t '⟼' t1" := (evaluate k t t1).
+
+(** *** Multi transition step with fuel *)
+
+Reserved Notation "k '⊨' t '⊢' st '⟶' t1" 
+                  (at level 57, t custom wh, t1 custom wh, no associativity).
+
+Inductive indexed : lvl -> nat -> Λ -> Λ -> Prop :=
+  | index_refl (lb : lvl) (t : Λ) : 
+  
+      (* ------------------ *)
+           lb ⊨ t ⊢ 0 ⟶ t
+
+  | index_step (lb : lvl) (k : nat) (t t1 t' : Λ) : 
+  
+           lb ⊨ t ⟼ t1 -> lb ⊨ t1 ⊢ k ⟶ t' -> 
+      (* -------------------------------------- *)
+                   lb ⊨ t ⊢(S k)⟶ t'
+
+where "k '⊨' t '⊢' st '⟶' t1" := (indexed k st t t1).
+
+(** *** Multi transition step *)
+Definition multi (k : lvl) :=  clos_refl_trans_1n Λ (evaluate k).
+
+
+Notation "k '⊨' t '⟼⋆' t1" := (multi k t t1) 
+                                (at level 57, t custom wh, t1 custom wh, no associativity).
+
+(** *** Halts *)
+Definition halts (k : lvl)  (t : Λ) : Prop :=  exists t', k ⊨ t ⟼⋆ t' /\  value(t').
+
+(** *** Normal form *)
+Definition normal_form (k : lvl) (t : Λ) : Prop := ~ (exists t', k ⊨ t ⟼ t').
+
+#[export] Hint Constructors evaluate clos_refl_trans_1n indexed : core.
+
+(** ---- *)
+
+(** ** Property - Evaluation *)
+
+(** *** [subst] property *)
+
+(** *** [evaluate] property *)
+
+(** *** [multi] property *)
+
+(** *** [halts] property *)
+
+(** ---- *)
+
+(** ** Preservation - Evaluation *)
+
+(** ---- *)
+
+(** ** Progress - Evaluation *)
